{"nbformat":4,"nbformat_minor":0,"metadata":{"kernelspec":{"display_name":"Python 3","language":"python","name":"python3"},"language_info":{"codemirror_mode":{"name":"ipython","version":3},"file_extension":".py","mimetype":"text/x-python","name":"python","nbconvert_exporter":"python","pygments_lexer":"ipython3","version":"3.6.8"},"colab":{"name":"ha3.ipynb","provenance":[],"collapsed_sections":[]}},"cells":[{"cell_type":"code","metadata":{"id":"ecxXfkuQ1eBq","colab_type":"code","colab":{}},"source":["import sympy as sp\n","import numpy as np\n","import matplotlib.pyplot as plt"],"execution_count":0,"outputs":[]},{"cell_type":"markdown","metadata":{"id":"kT-qJhS41eB1","colab_type":"text"},"source":["### 1. Derive formula of $L_{2}(x)$ in terms of interpolation phase $ u = \\frac{x - x_{i}}{h} $.  Integrate $ \\hat{I_{i}^{i+2}}$ with received formula as integrand  [mathematical formula]. Usetimation time: ~30m"]},{"cell_type":"markdown","metadata":{"id":"O4H3eBRY1eB7","colab_type":"text"},"source":["**Note** Use constant step $h = const$ and condition *number of segments is even* $n = 2k$"]},{"cell_type":"markdown","metadata":{"id":"p3_v3df_49Eq","colab_type":"text"},"source":["$L_2(x)=\\dfrac{(x-x_{i+1})(x-x_{i+2})}{(x_i-x_{i+1})(x_i-x_{i+2})}f_i + \\dfrac{(x-x_i)(x-x_{i+2})}{(x_{i+1}-x_i)(x_{i+1}-x_{i+2})}f_{i+1}+\\dfrac{(x-x_i)(x-x_{i+1})}{(x_{i+2}-x_i)(x_{i+2}-x_{i+1})}f_{i+2}$\n","\n","Since $h = const = x_{m+1}-x_m$\n","\n","$L_2(x)=\\dfrac{(x-x_{i+1})(x-x_{i+2})}{(-h)(-2h)}f_i + \\dfrac{(x-x_i)(x-x_{i+2})}{(h)(-h)}f_{i+1}+\\dfrac{(x-x_i)(x-x_{i+1})}{(2h)(h)}f_{i+2}$\n","\n","\n","$u=\\dfrac{(x-x_i)}{h}$\n","\n","\n","$\\dfrac{x-x_{i+1}}{h} = \\dfrac{x-x_i+x_i-x_{i+1}}{h}= \\dfrac{x-x_i-h}{h} = \\dfrac{x-x_i}{h} - 1 = u-1$\n","\n","$\\dfrac{x-x_{i+2}}{h} = \\dfrac{x-x_i+x_i-x_{i+2}}{h}= \\dfrac{x-x_i-2h}{h} = \\dfrac{x-x_i}{h} - 2 = u-2$\n","\n","$L_2(u)=\\dfrac{(u-1)(u-2)}{2}f_i - u(u-2)f_{i+1}+\\dfrac{u(u-1)}{2}f_{i+2}$\n","\n","$L_2(u)=\\dfrac{u^2-3u+2}{2}f_i - (u^2-2u)f_{i+1}+\\dfrac{u^2-u}{2}f_{i+2}$\n","\n","$u(x_i)=0,u(x_{i+2})=2$\n","\n","$\\int^{x_{i+2}}_{x_i}L_2(x)dx = \\int^{2}_{0}L_2(u)d(uh+x_i) =\\int^{2}_{0}L_2(u)hd(u)$\n","\n","$\\int^{2}_{0}(\\dfrac{u^2-3u+2}{2}f_i - (u^2-2u)f_{i+1}+\\dfrac{u^2-u}{2}f_{i+2})hdu=\n","((\\dfrac{u^3}{3}-\\dfrac{3u^2}{4}+u)f_i -(\\dfrac{u^3}{3}-u^2)f_{i+1}+ (\\dfrac{u^3}{6}-\\dfrac{u^2}{4})f_{i+2})h|^{2}_{0} =((\\dfrac{8}{6}-3+2)f_i-(\\dfrac{8}{3}-4)f_{i+1}+(\\dfrac{8}{6}-1)f_{i+2})h = \\dfrac{h}{3}f_i+\\dfrac{4}{3}f_{i+1}h+\\dfrac{h}{3}f_{i+2} = \\dfrac{h}{3} (f_{i} + 4f_{i+1} + f_{i+2})$\n","\n","\n"]},{"cell_type":"markdown","metadata":{"id":"JdZjxa5L1eCF","colab_type":"text"},"source":["### 2. Explain how used condition $n = 2k$ helps us in integration. If we want to use odd number of segments we have to integrate with even number of segments but add the value $I_{n-1}^n$. What is the calculation accuracy order of $I_{n-1}^n$? Why? Explain both. [mathematical formula]. Usetimation time: ~30m"]},{"cell_type":"markdown","metadata":{"id":"jw85ePWmN-RH","colab_type":"text"},"source":["1)For even number of segments n=2k calculate k pairs of segments.\n","\n","For odd number of segments n=2k+1 calculate k pairs of segments plus the last one:\n","$(X3 4to tbl xoteJl yBu9etb B otBete Ha CBou >|<e otBet B Bo||poce)$\n","\n","$\\hat I_{2k}^{2k+1} = \\hat I^{x_{2k+1}}_{x_{2k-2}}-\\hat I^{x_{2k}}_{x_{2k-2}}$\n","\n","2)Newton-Cotes formula coupled with Simpson's formula can provie O(h^5) estimation of the last segment\n","\n","$\\hat I^{x_{2k+1}}_{x_{2k-2}}-\\hat I^{x_{2k}}_{x_{2k-2}} = O(n^5)-O(n^5)$\n","\n"]},{"cell_type":"markdown","metadata":{"id":"-DFOJMJh1eCN","colab_type":"text"},"source":["### 3. Derive the formula of whole $\\hat{I_{a}^{b}}$. Summarize all integrals on segments $\\hat{I_{i}^{i+1}}$ for even case, and for odd case. [mathematical formula]. Usetimation time: ~30m"]},{"cell_type":"markdown","metadata":{"id":"ujNJBQMluQ7G","colab_type":"text"},"source":["$\\hat I_{x_i}^{x_{i+2}} =\\frac{h}{3} (f_{i} + 4f_{i+1} + f_{i+2})$\n","\n","$\\hat I_{x_i}^{x_{i+2k}} =\\sum_{j=0}^{k-1}\\frac{h}{3} (f_{2j} + 4f_{2j+1} + f_{2j+2})=$\n","\n","$\\frac{h}{3} (\\sum_{j=0}^{k-1}f_{2j} + 4\\sum_{j=0}^{k-1}f_{2j+1} + \\sum_{j=0}^{k-1}f_{2j+2})=$\n","$\\frac{h}{3} (\\sum_{j=1}^{k-1}f_{2j}+f_0 + 4\\sum_{j=0}^{k-1}f_{2j+1} + \\sum_{j=1}^{k-1}f_{2j}+f_{2k})=$\n","$\\frac{h}{3} (f_0 + 4\\sum_{j=0}^{k-1}f_{2j+1} + 2\\sum_{j=1}^{k-1}f_{2j}+f_{2k})$\n","\n","$\\hat I_{0}^{2k+1} = \\hat I_{0}^{2k} + \\hat I^{2k+1}_{2k} = \\frac{h}{3} (f_0 + 4\\sum_{j=0}^{k-1}f_{2j+1} + 2\\sum_{j=1}^{k-1}f_{2j}+f_{2k})+\\hat I^{x_{2k+1}}_{2k}$\n","\n","\n","With Newton-Cotes formula for last three segments\n","\n","$\\hat I^{x_{2k+1}}_{x_{2k-2}}=\\dfrac{3h}{8}(f_{2k-2}+3f_{2k-1}+3f_{2k}+f_{2k+1})$\n","\n","$\\hat I_{2k}^{2k+1} = \\hat I^{x_{2k+1}}_{x_{2k-2}}-\\hat I^{x_{2k}}_{x_{2k-2}} =$\n","$\\dfrac{3h}{8}(f_{2k-2}+3f_{2k-1}+3f_{2k}+f_{2k+1})-\\frac{h}{3} (f_{2k-2} + 4f_{2k-1} + f_{2k})= \\dfrac{9h}{24}(f_{2k-2}+3f_{2k-1}+3f_{2k}+f_{2k+1})-\\frac{8h}{24} (f_{2k-2} + 4f_{2k-1} + f_{2k}) = \\dfrac{h}{24}(f_{2k-2}-5f_{2k-1}+19f_{2k}+9f_{2k+1})$"]},{"cell_type":"markdown","metadata":{"id":"JCuxQius1eCX","colab_type":"text"},"source":["### 4. Derive the formula of trapezoid quadrature formula error estimation. Use Taylor series expansion for antiderivative $F_{i+1}$ and $f_{i+1}$  [mathematical formula] Usetimation time: ~30m"]},{"cell_type":"markdown","metadata":{"id":"F60xJtkebKDH","colab_type":"text"},"source":["$ I_i^{i+1} - \\hat I_{i,тр}^{i+1} = F_{i+1} - F_i - \\dfrac{h_{i+1}}{2}(f_i + f_{i+1}) = F_i + h_{i+1}f_i + \\dfrac{h_{i+1}^2}{2}f'_i + \\dfrac{h_{i+1}^3}{6}f''_i(\\xi_i) - F_i - \\dfrac{h_{i+1}}{2}(f_i + f_i + h_{i+1}f'_i + \\dfrac{h_{i+1}^2}{2}f''(\\xi_i)) = \\dfrac{h_{i+1}^3}{6}f''(\\xi_i) - \\dfrac{h_{i+1}^3}{4}f''(\\xi_i) = -\\dfrac{1}{12}h_{i+1}^3 f''(\\xi_i) $"]},{"cell_type":"markdown","metadata":{"id":"asVKyBVX1eCg","colab_type":"text"},"source":["### Congrats!"]}]}